some lemmas proved

proof/model.v
@@ -1,56 +1,492 @@
-Require Import Bool Arith List Lia List.
+Require Import Bool Arith List Lia List String.
+Require Import Lists.List.
+Import ListNotations.
 
-(* Execution mode *)
+(* Execution modes *)
 Inductive mode : Type := 
   | NormalMode
-  | EnclaveMode 
+  | EnclaveMode (* maybe we should have another critical mode! *)
 .
 
-(* Different types of memory regions *)
+(* Abstract Memory model *)
+
+(* Content stored in the memory *)
 
 Inductive enc_mem_tag : Type :=
   | ZoneMem
   | NonzoneMem
 .
 
+Inductive security_tag : Type :=
+  | Secret
+  | Declassified
+  | Nonsense
+.
+
+Definition sum_two_tags (t1 t2: security_tag) : security_tag := 
+  match t1 with
+  | Nonsense => Nonsense
+  | Secret => match t2 with
+              | Nonsense => Nonsense
+              | _ => Secret
+              end
+  
+  | Declassified => match t2 with
+              | Nonsense => Nonsense
+              | Secret => Secret
+              | Declassified => Declassified
+              end
+  end.
+
 Inductive value : Type :=
-  | Concrete (v: nat) (* This may not be a nat here? *)
+  | ConcreteN (v: nat) (* This may not be a nat here? *)
+  | ConcreteB (v: bool)
   | Any
 .
 
-Inductive accessible : Type :=
-  | Some (v: value)
-  | Uninit  (* uninitialized memory *)
-  | Error (* priviledge error *)
+Inductive location : Type :=
+  | Stack (n: nat) (* the stack should be bounded! *)
+  | Ident (s: string)
+  | RV
 .
 
-Inductive mem: Type :=
-  | AppMem (v: value)
-  | UnusedMem
-  | EncMem (z: enc_mem_tag) (v: value)
-.
-
-(* Memory and mappings *)
-
-(* Do we really need locations? Maybe we just need variable names (identifiers)? *)
-Definition location : Type := nat.
-
-(* Convention: location 0 ~ 15 are for registers *)
-Definition memory_mapping := location -> mem.
-
-Definition empty_mem (l: location) : memory_mapping := 
-  (fun _ => UnusedMem).
-
-Definition take_mem (me: mem) (mo: mode) : accessible :=
-  match me, mo with
-  | UnusedMem, _ => Uninit
-  | (EncMem _ _), NormalMode => Error
-  | (EncMem _ v), EnclaveMode => Some v
-  | AppMem v, _ => Some v
+Definition eq_location (i1 i2: location) : bool := 
+  match i1, i2 with
+  | Stack n1, Stack n2 => n1 =? n2
+  | Ident s1, Ident s2 => if string_dec s1 s2 then true else false
+  | RV, RV => true
+  | _, _ => false
   end.
 
-Definition update_mem (mm: memory_mapping) (l: location) (m: mem) : memory_mapping := 
-  fun l' => if l =? l' then m else mm l.
+Theorem eq_location_eq: forall i1 i2, eq_location i1 i2 = true <-> i1 = i2.
+Proof.
+  split. 
+  - destruct i1 eqn:eqi1; destruct i2 eqn:eqi2; unfold eq_location; 
+    intros; try discriminate H.
+    + apply beq_nat_true in H. rewrite H. reflexivity.
+    + destruct (string_dec s s0) as [Hs_eq | Hs_not_eq]. subst. reflexivity. discriminate H.
+    + reflexivity.
+  - destruct i1 eqn:eqi1; destruct i2 eqn:eqi2; unfold eq_location; 
+    intros; try discriminate H.
+    + apply Nat.eqb_eq. inversion H. reflexivity.
+    + destruct (string_dec s s0) as [Hs_eq | Hs_not_eq]. reflexivity. inversion H.
+      unfold not in Hs_not_eq. apply Hs_not_eq in H1. destruct H1. 
+    + reflexivity.
+Qed.
+
+Theorem eq_location_ne: forall i1 i2, eq_location i1 i2 = false <-> i1 <> i2.
+Proof.
+  split.
+  - unfold not. intros. apply eq_location_eq in H0. rewrite H0 in H. discriminate H.
+  - unfold not. intros.
+  destruct i1 eqn:eqi1; destruct i2 eqn:eqi2; unfold eq_location; try reflexivity.
+    + destruct (n =? n0) eqn: eqn0. apply Nat.eqb_eq in eqn0. subst. destruct H. reflexivity. reflexivity.
+    + destruct (string_dec s s0). subst. destruct H. reflexivity. reflexivity.
+    + destruct H. reflexivity. 
+Qed.
+
+Lemma eq_location_refl: forall (l: location), eq_location l l = true.
+Proof.
+  intros l. assert (H: l = l). reflexivity.
+  apply eq_location_eq. reflexivity.
+Qed.
+
+Definition tagged_value: Type := prod value security_tag.
+
+Definition tagged_value_example: tagged_value := (Any, Secret).
+
+Inductive cell: Type :=
+  | AppMem (v: tagged_value)
+  | UnusedMem (* may not need this! *)
+  | EncMem (z: enc_mem_tag) (v: tagged_value)
+.
+
+Definition cell_example1: cell := AppMem tagged_value_example.
+
+Definition cell_example2: cell := EncMem ZoneMem tagged_value_example.
+
+(* Result, memory, mapping, and accessing *)
+
+Inductive error: Type := 
+  | Invalid
+  | NoPriviledge
+.
+
+Definition errors: Type := list error.
+
+Inductive result {X: Type} : Type :=
+  | Ok (v: X)
+  | Err (e: errors)
+.
+
+Definition memory: Type := location -> cell.
+
+Definition empty_mem (l: location) : memory := 
+  (fun _ => UnusedMem).
+
+Definition eqb_string (x y : location) : bool :=
+  if eq_location x y then true else false.
+
+Definition update (s: location) (v: cell) (m: memory) : memory := 
+  fun s' => if (eq_location s' s) then v else m s'.
+
+(* raw_* is designed for security monitor, and should not be used in *)
+Definition raw_access (me: memory) (s: location) : option tagged_value := 
+  match me s with
+  | AppMem v => Some v
+  | EncMem _ v => Some v
+  | UnusedMem => None
+  end.
+
+(* Normal access doens't have restriction on reading to the Zone *)
+Definition access' (me: memory) (mo: mode) (s: location) : @result tagged_value := 
+  let c := me s in
+    match mo, c with
+    | _, UnusedMem => Err([Invalid])
+    | EnclaveMode, AppMem v
+    | EnclaveMode, EncMem _ v => Ok(v)
+    | NormalMode, EncMem _ _ => Err([NoPriviledge])
+    | NormalMode, AppMem v => Ok(v)
+    end.
+
+Definition access (me: memory) (mo: mode) (s: location) : @result tagged_value := 
+  let c := me s in
+    match mo, c with
+    | _, UnusedMem => Err([Invalid])
+    | EnclaveMode, AppMem v
+    | EnclaveMode, EncMem _ v => Ok(v)
+    | NormalMode, EncMem _ _ => Err([NoPriviledge])
+    | NormalMode, AppMem v => Ok(v)
+    end.
+
+(* Abstract Syntax: Expressions *)
+
+(* Inductive oprand: Type :=
+  | OpLoc (l: location) (* secret level dependet *)
+  | OpVal (v: value)    (* secret level always normal *)
+. *)
+
+Inductive exp: Type :=
+  | ExpLoc (l: location)
+  | ExpVal (v: value)
+  | ExpUnary (e: exp) (op: value -> value)
+  | ExpBinary (e1 e2: exp) (op: value -> value -> value)
+.
+
+(* Expression evaluation *)
+
+
+Fixpoint exp_prop_tag (me: memory) (mo: mode) (e: exp) : security_tag := 
+  match e with
+  | ExpLoc l => match access me mo l with
+                | Ok v => (snd v)
+                | Err e => Nonsense
+                end
+  | ExpVal v => Declassified
+  | ExpUnary e _ => exp_prop_tag me mo e
+  | ExpBinary e1 e2 _ =>  let t1 := exp_prop_tag me mo e1 in
+                          let t2 := exp_prop_tag me mo e2 in
+                          sum_two_tags t1 t2
+  end.
+
+(* bool evaluation *)
+
+(* NOT use in interpretation! *)
+Fixpoint raw_exp_eval (me: memory) (e: exp) : @result value := 
+  match e with
+  | ExpLoc l => match raw_access me l with
+                | Some v => Ok(fst v)
+                | None => Err([Invalid])
+                end
+  | ExpVal v => Ok(v)
+  | ExpUnary e _ => match raw_exp_eval me e with
+                    | Ok _ => Ok(Any)
+                    | Err er => Err(er)
+                    end
+  | ExpBinary e1 e2 _ => let r1 := raw_exp_eval me e1 in
+                         let r2 := raw_exp_eval me e2 in
+                         match r1, r2 with
+                         | Ok _, Ok _ => Ok(Any)
+                         | Err er1, Err er2 => Err(er1 ++ er2)
+                         | Err er1, Ok _ => Err(er1)
+                         | Ok _, Err er2 => Err(er2)
+                         end
+  end.
+
+Fixpoint exp_eval (me: memory) (mo: mode) (e: exp) : @result value := 
+  match e with
+  | ExpLoc l => match access me mo l with
+                | Ok v => Ok (fst v)
+                | Err e => Err e
+                end
+  | ExpVal v => Ok(v)
+  | ExpUnary e _ => match exp_eval me mo e with
+                    | Ok _ => Ok(Any)
+                    | e => e
+                    end
+  | ExpBinary e1 e2 _ => let r1 := exp_eval me mo e1 in
+                         let r2 := exp_eval me mo e2 in
+                         match r1, r2 with
+                         | Ok _, Ok _ => Ok(Any)
+                         | Err er1, Err er2 => Err(er1 ++ er2)
+                         | Err er1, Ok _ => Err(er1)
+                         | Ok _, Err er2 => Err(er2)
+                         end
+  end.
+
+Definition exp_tagged_val (me: memory) (mo: mode) (e: exp) : @result tagged_value := 
+  match (exp_eval me mo e), (exp_prop_tag me mo e) with
+  | Ok v, t => Ok (v, t)
+  | Err ev, _ => Err ev
+  end.
+
+
+(* bool evaluation *)
+
+Definition value_as_bool (v: value) : bool := 
+  match v with
+  | ConcreteN n => match n with
+                  | 0 => true
+                  | S _ => false
+                  end
+  | ConcreteB b => b
+  | Any => false
+  end.
+
+Definition exp_as_bool (me: memory) (mo: mode) (e: exp) : @result bool := 
+  match exp_eval me mo e with
+  | Ok v => Ok (value_as_bool v)
+  | Err e => Err e
+  end.
+
+
+(* NOT use in interpretation!
+Fixpoint raw_exp_as_bool (me: memory) (e: exp) : @result bool := 
+  match e with
+  | ExpLoc l => match raw_access me l with
+                | Some v => Ok(value_as_bool v)
+                | None => Err([Invalid])
+                end
+  | ExpVal v => Ok(value_as_bool v)
+  | ExpUnary e _ => match raw_exp_as_bool me e with
+                    | Ok _ => Ok(false)
+                    | Err er => Err(er)
+                    end
+  | ExpBinary e1 e2 _ => let r1 := raw_exp_as_bool me e1 in
+                         let r2 := raw_exp_as_bool me e2 in
+                         match r1, r2 with
+                         | Ok _, Ok _ => Ok(false)
+                         | Err er1, Err er2 => Err(er1 ++ er2)
+                         | Err er1, Ok _ => Err(er1)
+                         | Ok _, Err er2 => Err(er2)
+                         end
+  end.
+
+Fixpoint exp_as_bool (me: memory) (mo: mode) (e: exp) : @result bool := 
+  match e with
+  | ExpLoc l => match access me mo l with
+                | Ok v => Ok (value_as_bool (fst v))
+                | Err e => Err e
+                end
+  | ExpVal v => Ok(value_as_bool v)
+  | ExpUnary e _ => match exp_as_bool me mo e with
+                    | Ok _ => Ok(false)
+                    | e => e
+                    end
+  | ExpBinary e1 e2 _ => let r1 := exp_as_bool me mo e1 in
+                         let r2 := exp_as_bool me mo e2 in
+                         match r1, r2 with
+                         | Ok _, Ok _ => Ok(false)
+                         | Err er1, Err er2 => Err(er1 ++ er2)
+                         | Err er1, Ok _ => Err(er1)
+                         | Ok _, Err er2 => Err(er2)
+                         end
+  end. *)
+
+(* Abstract Syntax: Statements (commands) *)
+
+Inductive com : Type :=
+  | CNop
+  | CEenter
+  | CEexit
+  | CAsgn (l: location) (v: exp)
+  | CSeq (c1 c2: com)
+  | CIf (b: exp) (c1 c2: com)
+  | CWhile (b: exp) (c: com)
+  (* Declasification *)
+.
+
+(* State Machine
+Record State := {
+  mo: mode;
+  me: memory;
+  vars: list location;
+  er: errors;
+}.
+
+About State. *)
+
+Definition accessible: Type := list location.
+
+
+Definition procedure: Type := com.
+
+
+Fixpoint leaked (me: memory) (vars: accessible) : bool := 
+  match vars with
+  | [] => false
+  | l::ls => match me l with
+            (* secrets cannot stay on AppMem or nonzone EncMem *)
+            | AppMem (_, Secret) => true
+            | EncMem NonzoneMem (_, Secret) => true
+            | _ => leaked me ls
+            end
+  end.
+
+Lemma leaked_no_leak: forall (me: memory) (vars: accessible) (l: location) (tv: tagged_value),
+  leaked me vars = false -> In l vars -> raw_access me l = Some tv -> 
+  me l = AppMem tv \/ me l = EncMem NonzoneMem tv -> ~(snd tv = Secret).
+Proof.
+  intros. generalize dependent l. generalize dependent tv. induction vars.
+  - intros. simpl in *. destruct H0.
+  - unfold not in *. unfold raw_access in *. intros. apply IHvars with tv l.
+    + simpl in *. destruct (me a) eqn: eqa. destruct v. destruct s eqn: eqs.
+      * discriminate H.
+      * assumption.
+      * assumption.
+      * assumption.
+      * destruct H0.
+        -- (* a=l*)
+          destruct z. assumption. destruct v. destruct s. discriminate H. assumption. assumption.
+        -- (* In l vars *)
+          destruct z. assumption. destruct v. destruct s. discriminate H. assumption. assumption.
+    + destruct H0.
+      * subst. destruct H2; simpl in H; rewrite H0 in *; destruct tv; simpl in *; subst; discriminate H.
+      * assumption.
+    + assumption.
+    + assumption.
+    + assumption.
+Qed.
+  
+Lemma leaked_update: forall (me: memory) (vars: accessible) (l: location) (tv: tagged_value),
+  leaked me vars = false -> leaked (update l (EncMem ZoneMem tv) me) vars = false.
+Proof.
+  intros. generalize dependent l. generalize dependent tv. generalize dependent H. induction vars.
+  - simpl. reflexivity.
+  - destruct (me a) eqn:eqa. destruct v eqn:eqv. destruct s eqn:eqs.
+    + simpl. rewrite eqa. intros. discriminate H.
+    + simpl. rewrite eqa. intros. destruct (eq_location a l) eqn: eqal. apply eq_location_eq in eqal.
+    (* can be simpler *)
+      * subst. unfold update. rewrite eq_location_refl. apply IHvars with tv l in H. unfold update in H. assumption.
+      * subst. unfold update. rewrite eqal. rewrite eqa. apply IHvars with tv l in H. unfold update in H. assumption.
+    + simpl. rewrite eqa. intros. apply IHvars with tv l in H.  destruct (eq_location a l) eqn: eqal;
+      unfold update; unfold update in H.
+      * rewrite eqal. assumption.
+      * rewrite eqal. rewrite eqa. assumption.
+    + simpl. rewrite eqa. intros. apply IHvars with tv l in H.  destruct (eq_location a l) eqn: eqal;
+      unfold update; unfold update in H.
+      * rewrite eqal. assumption.
+      * rewrite eqal. rewrite eqa. assumption.
+    + simpl. rewrite eqa. destruct z eqn: eqz. intros. apply IHvars with tv l in H. destruct (eq_location a l) eqn: eqal; unfold update in *; rewrite eqal.
+      * assumption.
+      * rewrite eqa. assumption.
+      * destruct v. destruct s eqn: eqs; intros; try discriminate H; apply IHvars with tv l in H; unfold update in *; destruct (eq_location a l) eqn: eqal; try rewrite eqa; try assumption; try assumption.
+Qed.
+
+(* We regard all the arguments to a procedure are passed through stack *)
+(* should they also lie on the zoen? *)
+Fixpoint is_critical (me: memory) (vars: accessible) : bool :=
+  match vars with
+  | [] => false
+  | h :: t => match h with
+              | Stack n => match me h with
+                          | EncMem ZoneMem (_, Secret) => true
+                          | _ => is_critical me t
+                            end
+              | _ => is_critical me t
+              end
+  end.
+
+(* for critical procedures, secrects need to lay in the Zone *)
+
+
+Definition state: Type := memory * mode * accessible * errors.
+
+(* Semantics *)
+
+Check (length).
+
+(* interpreter for cirtcal procedures *)
+Inductive com_eval_critical : com -> state -> state -> Prop :=
+  | E_Err_ignore (me me': memory) (mo mo': mode) (vars vars': accessible) (ers ers': errors) 
+    (Her: (length ers) >= 1) (c: com):
+    com_eval_critical c (me, mo, vars, ers) (me', mo', vars', ers')
+  | E_Nop (st: state) (ers: errors): 
+    com_eval_critical CNop st st
+  | E_Eenter (me: memory) (mo: mode) (vars: accessible) (ers: errors) (Her: ers = []):
+    com_eval_critical CEenter (me, mo, vars, ers) (me, EnclaveMode, vars, ers)
+  | E_Eexit (me: memory) (mo: mode) (vars: accessible) (ers: errors) (Her: ers = []):
+    com_eval_critical CEexit (me, mo, vars, ers) (me, NormalMode, vars, ers)
+  | E_Asgn_Ok (me: memory) (mo: mode) (vars: accessible) (ers: errors) (Her: ers = [])
+    (l: location) (v: exp) (r: tagged_value) (Hexp: exp_tagged_val me mo v = (Ok r)):
+    (* Write restricted in the Zone! *)
+    com_eval_critical (CAsgn l v) (me, mo, vars, ers) ((update l (EncMem ZoneMem r) me), mo, (l :: vars), ers)
+  | E_Asgn_Err (me: memory) (mo: mode) (vars: accessible) (ers: errors) (Her: ers = [])
+    (l: location) (v: exp) (er: errors) (Hexp: exp_tagged_val me mo v = (Err er)):
+    com_eval_critical (CAsgn l v) (me, mo, vars, ers) (me, mo, vars, (er ++ ers))
+  | E_Seq (st st' st'': state) (c1 c2: com)
+    (Hc1: com_eval_critical c1 st st') (Hc2: com_eval_critical c2 st' st''):
+    com_eval_critical (CSeq c1 c2) st st''
+  | E_If_then (me: memory) (mo: mode) (vars: list location) (ers: errors) (Her: ers = [])
+    (b: exp) (c1 c2: com) (st': state):
+    exp_as_bool me mo b = Ok true -> 
+    com_eval_critical c1 (me, mo, vars, ers) st' -> 
+    com_eval_critical (CIf b c1 c2) (me, mo, vars, ers) st'
+  | E_If_else (me: memory) (mo: mode) (vars: list location) (ers: errors) (Her: ers = [])
+    (b: exp) (c1 c2: com) (st': state):
+    exp_as_bool me mo b = Ok false -> 
+    com_eval_critical c2 (me, mo, vars, ers) st' -> 
+    com_eval_critical (CIf b c1 c2) (me, mo, vars, ers) st'
+  | E_If_err (me: memory) (mo: mode) (vars: list location) (ers: errors) (Her: ers = [])
+    (b: exp) (c1 c2: com) (st': state) (er: errors):
+    exp_as_bool me mo b = Err er -> 
+    com_eval_critical (CIf b c1 c2) (me, mo, vars, ers) (me, mo, vars, er ++ ers)
+  | E_while_true (me: memory) (mo: mode) (vars: list location) (ers: errors) (Her: ers = [])
+    (b: exp) (c: com) (st': state):
+    exp_as_bool me mo b = Ok true -> 
+    com_eval_critical c (me, mo, vars, ers) st' -> 
+    com_eval_critical (CWhile b c) (me, mo, vars, ers) st'
+  | E_while_false (me: memory) (mo: mode) (vars: list location) (ers: errors) (Her: ers = [])
+    (b: exp) (c: com) (st': state):
+    exp_as_bool me mo b = Ok false -> 
+    com_eval_critical (CWhile b c) (me, mo, vars, ers) (me, mo, vars, ers)
+  | E_while_err (me: memory) (mo: mode) (vars: list location) (ers: errors) (Her: ers = [])
+    (b: exp) (c: com) (st': state) (er: errors):
+    exp_as_bool me mo b = Err er -> 
+    com_eval_critical (CWhile b c) (me, mo, vars, ers) (me, mo, vars, er ++ ers)
+.
+
+Lemma error_ignore : forall (me: memory) (mo: mode) (vars: accessible) (ers: errors) (c: com),
+  ((length ers) >= 1) -> com_eval_critical c (me, mo, vars, ers) (me, mo, vars, ers).
+Proof.
+  intros. constructor. assumption.
+Qed.
+
+Theorem restricted_no_leakage_proc: forall (me me': memory) (mo mo': mode) (vars vars': accessible) (ers ers': errors) (c: com),
+  leaked me vars = false -> is_critical me vars = true ->
+  com_eval_critical c (me, mo, vars, ers) (me', mo', vars', ers') ->
+  leaked me' vars' = false.
+Proof.
+  intros. induction H1.
+   inversion H1; subst; try assumption.
+  - apply leaked_update. simpl. 
+    + destruct (me l) eqn: eql. destruct v0. destruct s eqn: eqs. subst.
+Qed.
+
+
+(* Procedure(functionn) and task *)
+
+Definition procedure := list com.
 
 
 (* Fixpoint deref (m: mem_layout) (l: location) : tag_value :=
@@ -81,15 +517,7 @@ Definition test_memory_layout = []. *)
 (* We model the instructions in a more abstract way *)
 
 (* TODO: jumps, branches, ref, [loops] *)
-Inductive instr : Type :=
-  | nop
-  | copy (ld: location) (ls: location) (* actually copy value ld <- ls *)
-  | wirtev (l: location) (v: value)
-  | unaryop (l: location) (op: nat -> nat)
-  | binaryop (l1: location) (l2: location) (op: nat -> nat -> nat)
-  | eexit
-  | eenter
-.
+
 
 (* How to say a procedure is critical? *)
 
